Add some fixes and rename some Lemmas in Theorem

Vcg.v
@@ -82,7 +82,7 @@ End Assn_b.
 
 Import Assn_b.
 
-(** Defintion of a verification condition generator **)
+(** Definition of a verification condition generator **)
 
 Fixpoint tc (c : com) (m : Sigma.sigma)
             (cl: Phi.phi) (suite : assertion) : Prop :=
@@ -214,16 +214,16 @@ Qed.
 (** Verification of trivial procedure contract **)
 
 Parameter f : Proc.t.
-Definition cli_1 (x': Proc.t) :=
+Definition f_psi (x': Proc.t) :=
         if Proc.eqb x' f then CSkip else Psi.empty_psi x'.
 
-Definition phi_1 (x': Proc.t) :=
+Definition f_phi (x': Proc.t) :=
         if Proc.eqb x' f then empty_clause else Phi.empty_phi x'.
 
-Example tc_p_update : tc_p cli_1 phi_1.
+Example tc_p_update : tc_p f_psi f_phi.
 Proof.
 unfold tc_p.
-unfold cli_1, phi_1.
+unfold f_psi, f_phi.
 intros.
 destruct (Proc.eqb f0 f).
 - split.
